Batteries/Lean/SatisfiesM.lean
@@ -1,0 +1,28 @@
+/-
+Copyright (c) 2024 Lean FRO, LLC. All rights reserved.
+Released under Apache 2.0 license as described in the file LICENSE.
+Authors: Kim Morrison
+-/
+import Batteries.Classes.SatisfiesM
+import Lean.Elab.Command
+
+/-!
+# Construct `Satisfying` instances for the Lean monad stack.
+-/
+
+open Lean Elab Term Tactic Command
+
+instance : Satisfying CoreM :=
+  inferInstanceAs <| Satisfying (ReaderT _ <| StateRefT' _ _ (EIO _))
+
+instance : Satisfying MetaM :=
+  inferInstanceAs <| Satisfying (ReaderT _ <| StateRefT' _ _ CoreM)
+
+instance : Satisfying TermElabM :=
+  inferInstanceAs <| Satisfying (ReaderT _ <| StateRefT' _ _ MetaM)
+
+instance : Satisfying TacticM :=
+  inferInstanceAs <| Satisfying (ReaderT _ $ StateRefT' _ _ TermElabM)
+
+instance : Satisfying CommandElabM :=
+  inferInstanceAs <| Satisfying (ReaderT _ $ StateRefT' _ _ (EIO _))
