BatteriesTest/satisfying.lean
@@ -1,0 +1,21 @@
+import Batteries.Lean.SatisfiesM
+import Batteries.Data.Array.Monadic
+
+open Lean Meta Array Elab Term Tactic Command
+
+-- For now these live in the test file, as it's not really clear we want people relying on them!
+instance : LawfulMonad (EIO ε) := inferInstanceAs <| LawfulMonad (EStateM _ _)
+instance : LawfulMonad CoreM :=
+  inferInstanceAs <| LawfulMonad (ReaderT _ <| StateRefT' _ _ (EIO Exception))
+instance : LawfulMonad MetaM :=
+  inferInstanceAs <| LawfulMonad (ReaderT _ <| StateRefT' _ _ CoreM)
+instance : LawfulMonad TermElabM :=
+  inferInstanceAs <| LawfulMonad (ReaderT _ <| StateRefT' _ _ MetaM)
+instance : LawfulMonad TacticM :=
+  inferInstanceAs <| LawfulMonad (ReaderT _ $ StateRefT' _ _ $ TermElabM)
+instance : LawfulMonad CommandElabM :=
+  inferInstanceAs <| LawfulMonad (ReaderT _ $ StateRefT' _ _ $ EIO _)
+
+example (xs : Array Expr) : MetaM { ts : Array Expr // ts.size = xs.size } := do
+  let r ← satisfying (xs.mapM inferType) (size_mapM _ _)
+  return r
